Cleanup

SimAsm/SimAsm_Rules.thy
@@ -63,13 +63,8 @@ lift_definition vm_rel_of_ts_rel :: "('r,'v,'a) tstack rel \<Rightarrow> ('r,'v,
 lift_definition ts_rel_of_vm_rel :: "('r,'v,'a) varmap' rel \<Rightarrow> ('r,'v,'a) tstack rel" is 
   "\<lambda>x. {(s,s') | s s'. (vm_of_ts s,vm_of_ts s') \<in> x}".
   
-fun ts_lang_of_vm_lang :: "('r,'v,('r,'v,'a)varmap','a) lang \<Rightarrow> ('r, 'v, ('r, 'v, 'a) tstack, 'a) lang" where
-  "ts_lang_of_vm_lang (Skip) = Skip " |
-  "ts_lang_of_vm_lang (Op pred op auxfn) = Op (ts_pred_of_vm_pred pred) op (auxfn \<circ> vm_of_ts)" |
-  "ts_lang_of_vm_lang (SimAsm.lang.Seq a b) = SimAsm.lang.Seq (ts_lang_of_vm_lang a) (ts_lang_of_vm_lang b) " |
-  "ts_lang_of_vm_lang (If c t f) = If c (ts_lang_of_vm_lang t) (ts_lang_of_vm_lang f)" |
-  "ts_lang_of_vm_lang (While b Imix Ispec c) = While b (ts_pred_of_vm_pred Imix) (ts_pred_of_vm_pred Ispec) (ts_lang_of_vm_lang c) " |
-  "ts_lang_of_vm_lang (DoWhile Imix Ispec c b) = DoWhile (ts_pred_of_vm_pred Imix) (ts_pred_of_vm_pred Ispec) (ts_lang_of_vm_lang c) b "
+
+
 
 (*
 fun vm_lang_of_ts_lang :: "('r,'v,('r,'v,'a)tstack,'a) lang \<Rightarrow> ('r, 'v, ('r, 'v, 'a) varmap', 'a) lang" where
@@ -131,44 +126,49 @@ text \<open>
 Combine the base frame and the varmap projection into a labelled varmap, along with an invariant
 constraining the state to be speculative and fixing the captured variable set.\<close>
 lift_definition spec_pred_of_lvm_pred :: "('r,'v,'a) lvarmap' pred \<Rightarrow> 'r set \<Rightarrow> ('r,'v,'a) tstack pred" is
-  "\<lambda>P w. {ts | ts. mk_lvarmap (tstack_base ts) (vm_of_ts ts) \<in> P \<and> ts_is_spec ts \<and> w = capped ts}".
+  "\<lambda>P w. {ts | ts. mk_lvarmap (tstack_base ts) (vm_of_ts ts) \<in> P \<and> ts_is_spec ts \<and> w = topcapped ts \<and> w = capped ts}".
+
+lift_definition spec_pred_of_lvm_pred2 :: "('r,'v,'a) lvarmap' pred \<Rightarrow> ('r,'v,'a) tstack pred" is
+  "\<lambda>P. {ts | ts. mk_lvarmap (tstack_base ts) (vm_of_ts ts) \<in> P \<and> ts_is_spec ts}".
+
+fun op_vc
+  where
+    "op_vc (leak v e) pred = {ts. mk_lvarmap (tstack_base ts) (vm_of_ts ts) \<in> pred}" |
+    "op_vc op pred = {ts. ts_is_seq ts \<longrightarrow> mk_lvarmap (tstack_base ts) (vm_of_ts ts) \<in> pred}"
+
+fun ts_lang_of_vm_lang :: "('r,'v,('r,'v,'a)varmap',('r,'v,'a)lvarmap','a) lang \<Rightarrow> ('r, 'v, ('r, 'v, 'a) tstack,('r, 'v, 'a) tstack, 'a) lang" where
+  "ts_lang_of_vm_lang (Skip) = Skip " |
+  "ts_lang_of_vm_lang (Op pred op auxfn) = Op (op_vc op pred) op (auxfn \<circ> vm_of_ts)" |
+  "ts_lang_of_vm_lang (SimAsm.lang.Seq a b) = SimAsm.lang.Seq (ts_lang_of_vm_lang a) (ts_lang_of_vm_lang b) " |
+  "ts_lang_of_vm_lang (If c t f) = If c (ts_lang_of_vm_lang t) (ts_lang_of_vm_lang f)" |
+  "ts_lang_of_vm_lang (While b Imix Ispec c) = While b (ts_pred_of_vm_pred Imix) (spec_pred_of_lvm_pred2 Ispec) (ts_lang_of_vm_lang c) " |
+  "ts_lang_of_vm_lang (DoWhile Imix Ispec c b) = DoWhile (ts_pred_of_vm_pred Imix) (spec_pred_of_lvm_pred2 Ispec) (ts_lang_of_vm_lang c) b "
 
 text \<open>Constrain the base frame of a stack with a relation\<close>
 definition base_rel :: "('r,'v,'a) varmap' rel \<Rightarrow> ('r,'v,'a) tstack rel"
   where "base_rel R \<equiv> {(ts,ts'). (tstack_base ts,tstack_base ts') \<in> R}"
 
-text \<open>Constrain the base frame of a stack with a relation and constrain all subsequent frames with id\<close>
-definition base_rel_frame_id :: "('r,'v,'a) varmap' rel \<Rightarrow> ('r,'v,'a) tstack rel"
-  where "base_rel_frame_id R \<equiv> {(ts,ts') \<in> base_rel R. tstack_upper ts = tstack_upper ts'}"
+text \<open>Constrain the base frame of a stack with a relation and all subsequent frames with id\<close>
+definition base_rel_rely :: "('r,'v,'a) varmap' rel \<Rightarrow> ('r,'v,'a) tstack rel"
+  where "base_rel_rely R \<equiv> {(ts,ts') \<in> base_rel R. tstack_upper ts = tstack_upper ts'}"
 
 definition id_on
-  where "id_on w \<equiv> {(m,m'). (\<forall>v \<in> w. varmap_st m v = varmap_st m' v) \<and> varmap_rec.more m = varmap_rec.more m'}"
+  where "id_on w G \<equiv> { (ts,\<lparr>varmap_st = \<lambda>v. if v \<in> w then varmap_st ts v else varmap_st ts' v, 
+                            \<dots> = varmap_rec.more ts\<rparr>) | ts ts'. (ts,ts') \<in> G }"
 
 text \<open>
-Constrain the base frame of a stack with a relation and constrain the number of subsequent frames,
-but not their contents. Additionally, allow any behaviour in the event that there are not the
-expected number of frames.
-\<close>
-definition base_rel_frame_sz :: "('r,'v,'a) varmap' rel \<Rightarrow> nat \<Rightarrow> 'r set \<Rightarrow> ('r,'v,'a) tstack rel"
-  where "base_rel_frame_sz R n w \<equiv> {(ts,ts'). ((ts,ts') \<in> base_rel (R \<inter> id_on w) \<or> tstack_len ts \<noteq> n) \<and> tstack_len ts = tstack_len ts'}"
-
-definition base_rel_frame1 :: "('r,'v,'a) varmap' rel \<Rightarrow> ('r,'v,'a) tstack rel"
-  where "base_rel_frame1 R \<equiv> {(ts,ts'). ((ts,ts') \<in> base_rel R \<or> tstack_len ts \<noteq> 1) \<and> tstack_len ts = tstack_len ts'}"
-
-(*
-  Guarantee: varmap of one frame down is in G with w fixed
-    or just the G itself 
-
-*)
-
-definition fixed ::  "('r,'v,'a) varmap' rel \<Rightarrow> 'r set \<Rightarrow> ('r,'v,'a) varmap' rel"
-  where "fixed G w \<equiv> {(m, m'\<lparr> varmap_st := \<lambda>v. if v \<in> w then varmap_st m v else varmap_st m' v \<rparr>) | m m'. (m,m') \<in> G}"
-
-
-
+Constrain the base frame of a stack with a relation, all intermediate frames with id, 
+but only ensure the topmost frame retains its capture set\<close>
 definition base_rel_guar :: "('r,'v,'a) varmap' rel \<Rightarrow> 'r set \<Rightarrow> ('r,'v,'a) tstack rel"
-  where "base_rel_guar G w \<equiv> {(ts,ts'). (ts,ts') \<in> base_rel G} \<inter> {(ts,ts'). tstack_len ts = tstack_len ts'}"
+  where "base_rel_guar G w \<equiv> {(ts,ts') \<in> base_rel G. ts_is_seq ts \<and> ts_is_seq ts'} \<union>
+                              {(ts,ts') \<in> base_rel (id_on w G). ts_is_spec ts \<and>
+                                                    tstack_mid ts = tstack_mid ts' \<and> 
+                                                    topcapped ts = topcapped ts' \<and>
+                                                    tstack_len ts = tstack_len ts' }"
 
+definition lift_pred :: "('r,'v,'a) spec_state \<Rightarrow> ('r,'v,'a) tstack pred"
+  where "lift_pred P \<equiv> {ts. if ts_is_seq ts then ts \<in> ts_pred_of_vm_pred (snd P) 
+                             else mk_lvarmap (tstack_base ts) (vm_of_ts ts) \<in> (fst P)}"
 
 
 
@@ -182,7 +182,7 @@ The judgement over the sequential program behaviour, structured with:
 \<close>
 abbreviation seq_rule ("_,_ \<turnstile>\<^sub>; _ {_,_,_} _" [20,0,0,0,0,0,20] 20)
   where "seq_rule R G P c r w Q \<equiv> 
-          (base_rel_frame_id (step\<^sub>t R)), (base_rel_guar (step G) w) \<turnstile> 
+          (base_rel_rely (step\<^sub>t R)), (base_rel_guar (step G) w) \<turnstile> 
             (seq_pred_of_vm_pred P) {lift\<^sub>c (ts_lang_of_vm_lang c) r w} (seq_pred_of_vm_pred Q)"
 
 text \<open>
@@ -195,18 +195,19 @@ The judgement over the speculative program behaviour, structured with:
 \<close>
 abbreviation spec_rule ("_,_ \<turnstile>\<^sub>s _ {_,_,_} _" [20,0,0,0,0,0,20] 20)
   where "spec_rule R G P c r w Q \<equiv> 
-          (base_rel_frame_id (step\<^sub>t R)), (base_rel_guar G w) \<turnstile> 
+          (base_rel_rely (step\<^sub>t R)), (base_rel_guar (step G) w) \<turnstile> 
             (spec_pred_of_lvm_pred P w) {lift\<^sub>c (ts_lang_of_vm_lang c) r w} (spec_pred_of_lvm_pred Q w)"
 
 text \<open>Combine the above into a single rule\<close>
-abbreviation lifted_abv ("_,_,_ \<turnstile> _ {_,_,_} _" [20,0,0,0,0,0,0,20] 20)
-  where "lifted_abv R G G' P c r w Q \<equiv> (seq_rule R G [P]\<^sub>; c r w [Q]\<^sub>; \<and> spec_rule R G' [P]\<^sub>s c r w [Q]\<^sub>s)"
+abbreviation lifted_abv ("_,_ \<turnstile> _ {_,_,_} _" [20,0,0,0,0,0,20] 20)
+  where "lifted_abv R G P c r w Q \<equiv> (seq_rule R G [P]\<^sub>; c r w [Q]\<^sub>; \<and> spec_rule R G [P]\<^sub>s c r w [Q]\<^sub>s)"
 
 text \<open>Define validity in terms of the sequential rule\<close>
 abbreviation validity_abv ("\<Turnstile> _ SAT [_, _, _, _]" [60,0,0,0] 45) 
   where "validity_abv c P R G Q \<equiv> 
     validity (lift\<^sub>c (ts_lang_of_vm_lang c) com.Nil (wr\<^sub>l c)) (seq_pred_of_vm_pred P) 
-      (base_rel_frame_id (step\<^sub>t R)) (base_rel_guar (step G) (wr\<^sub>l c)) (seq_pred_of_vm_pred Q)" 
+      (base_rel_rely (step\<^sub>t R)) (base_rel_guar (step G) (wr\<^sub>l c)) (seq_pred_of_vm_pred Q)" 
+
 
 (*
 text \<open>An ordering property on contexts\<close>
@@ -241,7 +242,7 @@ lemma vm_of_ts_in_seq_pred_of_vm_pred[simp]:
   unfolding seq_pred_of_vm_pred_def by simp
 
 lemma vm_of_ts_in_spec_pred_of_vm_pred[simp]: 
-  "(x \<in> spec_pred_of_lvm_pred P w) = (mk_lvarmap (tstack_base x) (vm_of_ts x) \<in> P \<and> ts_is_spec x \<and> w = capped x)"
+  "(x \<in> spec_pred_of_lvm_pred P w) = (mk_lvarmap (tstack_base x) (vm_of_ts x) \<in> P \<and> ts_is_spec x \<and> w = capped x \<and> w = topcapped x)"
   by (auto simp: spec_pred_of_lvm_pred_def)
 
 lemma seq_ts_mono:
@@ -287,40 +288,36 @@ subsection \<open>Relational @{type tstack} Projection Lemmas\<close>
 
 lemma stable\<^sub>L [intro]:
   assumes "stable\<^sub>L R P"
-  shows "stable (base_rel_frame_id (step\<^sub>t R)) (spec_pred_of_lvm_pred P w)"
+  shows "stable (base_rel_rely (step\<^sub>t R)) (spec_pred_of_lvm_pred P w)"
   sorry (* Problem 1: Stability in the speculative context doesn't make sense *)
 
+lemma stabilize\<^sub>L_entail:
+  "t \<in> stabilize\<^sub>L R P \<Longrightarrow> reflexive R \<Longrightarrow> P \<subseteq> Q \<Longrightarrow> t \<in> stabilize\<^sub>L R Q"
+  sorry (* Problem *) 
+
 lemma stable_ts [intro]: 
-  "stable R P \<Longrightarrow> stable (base_rel_frame_id R) (seq_pred_of_vm_pred P)"
-  apply (auto simp: stable_def base_rel_frame_id_def base_rel_def )
+  "stable R P \<Longrightarrow> stable (base_rel_rely R) (seq_pred_of_vm_pred P)"
+  apply (auto simp: stable_def base_rel_rely_def base_rel_def )
   apply (metis One_nat_def tstack_base_vm_of_ts tstack_upper_len_eq)
   apply (metis tstack_upper_len_eq)
   done
 
-lemma base_rel_frame_szI1:
-  assumes "tstack_len a = 1 \<Longrightarrow> (tstack_base a, tstack_base b) \<in> G" "tstack_len a = tstack_len b"
-  shows "(a,b) \<in> base_rel_frame1 G"
-  using assms unfolding base_rel_frame1_def base_rel_def
-  by auto
-
-lemma base_rel_frame_szI:
-  assumes "tstack_len a = n \<Longrightarrow> (tstack_base a, tstack_base b) \<in> G \<inter> id_on w" "tstack_len a = tstack_len b"
-  shows "(a,b) \<in> base_rel_frame_sz G n w"
-  using assms unfolding base_rel_frame_sz_def base_rel_def
-  by auto
-
 lemma base_rel_guarI:
-  assumes "(tstack_base a, tstack_base b) \<in> G"
+  assumes "ts_is_seq a \<Longrightarrow> ts_is_seq b \<Longrightarrow> (tstack_base a, tstack_base b) \<in> G"
+  assumes "ts_is_spec a \<Longrightarrow> (tstack_base a, tstack_base b) \<in> id_on w G"
+  assumes "topcapped a = topcapped b"
+  assumes "tstack_mid a = tstack_mid b"
   assumes "tstack_len a = tstack_len b"
-  shows "(a,b) \<in> base_rel_guar G n"
+  shows "(a,b) \<in> base_rel_guar G w"
   using assms unfolding base_rel_guar_def base_rel_def
-  by auto
+  by fastforce
 
 lemma [elim!]:
   assumes "(tstack_push m s, tstack_push ma sa) \<in> base_rel G"
   obtains "(m, ma) \<in> base_rel G"
   using assms unfolding base_rel_def by auto
 
+(* MOVE *)
 lemma [intro]:
   assumes "tstack_upper m = tstack_upper m'"
   shows "tstack_upper (tstack_push m s) = tstack_upper (tstack_push m' s)"
@@ -330,10 +327,119 @@ lemma [simp]:
   "tstack_len m = 1 \<Longrightarrow> tstack_upper m = []"
   unfolding tstack_upper_def by transfer (case_tac m; simp)
 
+lemma butlast_topcap:
+  "butlast a = butlast b \<Longrightarrow> topcap a = topcap b"
+  unfolding topcap_def by (auto split: list.splits simp: fun_eq_iff)
+
+lemma tstack_upper_topcap:
+  "tstack_upper a = tstack_upper b \<Longrightarrow> ttopcap a = ttopcap b"
+  unfolding tstack_upper_def by transfer (rule butlast_topcap)
+
+lemma [simp]:
+  "tstack_len x = Suc 0 \<Longrightarrow> tcaptured x v = False"
+  by transfer (case_tac x; auto simp: captured_def)
+
+lemma [intro]:
+  "ttopcap x x11 \<Longrightarrow> tcaptured x x11"
+  by transfer (case_tac x; auto simp: captured_def topcap_def split: list.splits)
+
+lemma [simp]:
+  "ttopcap (tauxupd x f) = ttopcap x"
+  apply transfer
+  unfolding topcap_def auxupd_def
+  by (auto split: list.splits simp: fun_eq_iff)
+
+lemma [simp]:
+  "ttopcap (tupdate x  y e) = ttopcap x"
+  apply transfer
+  unfolding topcap_def auxupd_def
+  by (auto split: list.splits simp: fun_eq_iff)
+
+lemma upper_mid:
+  "tstack_upper a = tstack_upper b \<Longrightarrow>
+           tstack_mid a = tstack_mid b"
+  by (auto simp: tstack_upper_def tstack_mid_def split: list.splits if_splits)
+
+lemma tstack_mid_tauxupd [simp]:
+  "tstack_mid (tauxupd x f) = tstack_mid x"
+  unfolding tstack_mid_def
+  by transfer (auto simp: fun_eq_iff auxupd_def split: list.splits)
+
+lemma tstack_mid_tupdate_base[simp]:
+  "tstack_len x = Suc 0 \<Longrightarrow> tstack_mid (tupdate x y e) = tstack_mid x"
+  unfolding tstack_mid_def
+  by transfer (auto split: list.splits)
+
+lemma stack_mid_update_nocap:
+  "Is_tstack (x21 # x22) \<Longrightarrow>
+       \<not> captured (x21 # x22) y \<Longrightarrow>
+       butlast (update x22 y e) = butlast x22"
+proof (induct "x21 # x22" arbitrary: x21 x22 rule: Is_tstack_induct)
+  case (Base x)
+  then show ?case by auto
+next
+  case (Frame x xs)
+  then show ?case by (cases xs; auto simp: captured_def)
+qed
+
+lemma tstack_mid_tupdate_nocap[simp]:
+  "\<not>tcaptured x y \<Longrightarrow> tstack_mid (tupdate x y e) = tstack_mid x"
+  unfolding tstack_mid_def
+  apply transfer 
+  apply (auto split: list.splits)
+  using stack_mid_update_nocap by force
+
+lemma tstack_mid_tupdate_topcap[simp]:
+  "ttopcap x y \<Longrightarrow> tstack_mid (tupdate x y e) = tstack_mid x"
+  unfolding tstack_mid_def
+  by transfer (auto split: list.splits simp: topcap_def)
+
+
+lemma [simp]:
+  "tstack_mid (tstack_push m s) = tstack_upper m"
+  unfolding tstack_mid_def tstack_upper_def
+  apply transfer
+  apply (auto split: list.splits)
+  done
+
+lemma [simp]:
+  "ttopcap (tstack_push m (emptyFrame w)) x = (x \<in> w)"
+  by transfer
+   (auto simp: topcap_def split: list.splits)
+
+(* MOVE *)
+
 lemma compat_example:
   assumes "G \<subseteq> R"
-  shows "base_rel_frame1 G \<subseteq> guard {t. tstack_len t = 1} (base_rel_frame_id R)"
-  using assms by (auto simp: base_rel_frame1_def base_rel_frame_id_def base_rel_def guard_def)
+  shows "base_rel_guar G w \<subseteq> guard {t. tstack_len t = 1} (base_rel_rely R)"
+  using assms by (auto simp: base_rel_guar_def base_rel_rely_def base_rel_def guard_def)
+
+lemma [elim!]:
+  assumes "[] = tstack_upper b"
+  obtains "tstack_len b = 1"
+  using assms unfolding tstack_upper_def apply (transfer)
+  apply (case_tac b; auto split: if_splits)
+  done
+
+lemma base_rel:
+  assumes "id_on w G \<subseteq> G"
+  shows "base_rel_rely (id_on w G) \<subseteq> base_rel_guar G w"
+  using assms
+  apply (auto simp: base_rel_rely_def base_rel_guar_def)
+               apply (simp add: base_rel_def subsetD)
+  using upper_mid apply blast
+  using tstack_upper_topcap apply force
+  using tstack_upper_topcap apply force
+  using tstack_upper_len_eq apply blast
+    using upper_mid apply blast
+  using tstack_upper_topcap apply force
+  using tstack_upper_topcap apply force
+  using tstack_upper_len_eq apply blast
+    using upper_mid apply blast
+  using tstack_upper_topcap apply force
+  using tstack_upper_topcap apply force
+  using tstack_upper_len_eq apply blast
+  done
 
 subsection \<open>@{term st_beh\<^sub>i} Invariants\<close>
 
@@ -361,34 +467,73 @@ method force_eq =
   (match conclusion in "f (a :: ('r, 'v, 'a) varmap_rec_scheme) = f b" for f a b \<Rightarrow>
     \<open>rule arg_cong[where ?f=f]\<close>)
 
+lemma u_lvarmap:
+  "v\<^sup>U = {x. mk_lvarmap ( x) ( x) \<in> v}"
+  unfolding restrict_pred_def mk_lvarmap_def image_def
+  apply auto
+   apply force_eq+
+  apply (rule exI)
+  apply (intro conjI)
+  prefer 2
+    apply blast
+   apply auto
+  done
+
 lemma [simp]:
-  "tstack_len x = Suc 0 \<Longrightarrow> tcaptured x v = False"
-  sorry
+  "(x, y) \<in> beh (lift\<^sub>b v op f) \<Longrightarrow> ttopcap x = ttopcap y"
+  by (cases op; auto simp: liftg_def)
+
+lemma id_on_refl :
+  assumes "(x,x) \<in> R"
+  shows "(x,x) \<in> (id_on w R)"
+  using assms unfolding id_on_def 
+  apply auto
+  apply (rule exI)
+  apply (intro conjI)
+  prefer 2
+   apply blast
+  apply auto
+  done
 
 lemma atomic_seq:
   assumes r: "wellformed R G"
-  assumes g: "(v \<subseteq> guar (wp\<^sub>i op o wp\<^sub>a f) (step G))"
+  assumes g: "v\<^sup>U \<subseteq> guar (wp\<^sub>i op o wp\<^sub>a f) (step G)"
+  assumes g': "\<forall>m. v \<subseteq> {s. s \<in> wp\<^sub>i\<^sub>s op {t'. ((gl_restrict s)\<lparr> varmap_rec.more := m \<rparr>, gl_restrict t'\<lparr> varmap_rec.more := m \<rparr>) \<in> id_on w (step G)}}"
   assumes s: "stable (step\<^sub>t R) Q"
-  shows "R,G \<turnstile>\<^sub>; stabilize R (v \<inter> wp\<^sub>i op (wp\<^sub>a f Q)) {Op v op f,r,w} Q"
+  shows "R,G \<turnstile>\<^sub>; stabilize R (v\<^sup>U \<inter> wp\<^sub>i op (wp\<^sub>a f Q)) {Op v op f,r,w} Q"
   unfolding ts_lang_of_vm_lang.simps lift\<^sub>c.simps
 proof (intro basic atomicI, goal_cases st gu spre spost)
   case st
-  let ?lhs = "seq_pred_of_vm_pred (stabilize R (v \<inter> wp\<^sub>i op (wp\<^sub>a f Q)))"
-  have vc: "?lhs \<subseteq> vc (lift\<^sub>b (ts_pred_of_vm_pred v) op (f \<circ> vm_of_ts))"
-    using r by (cases op) (auto elim: stabilizeE intro!: seq_ts_mono simp: liftg_def)
-  have wp: "?lhs \<subseteq> {m. \<forall>m'. (m, m') \<in> beh (lift\<^sub>b (ts_pred_of_vm_pred v) op (f \<circ> vm_of_ts)) \<longrightarrow> 
+  let ?lhs = "seq_pred_of_vm_pred (stabilize R (v\<^sup>U \<inter> wp\<^sub>i op (wp\<^sub>a f Q)))"
+  have vc: "?lhs \<subseteq> vc (lift\<^sub>b (op_vc op v) op (f \<circ> vm_of_ts))"
+    using r by (cases op) (auto elim: stabilizeE intro!: seq_ts_mono simp: liftg_def u_lvarmap)
+  have wp: "?lhs \<subseteq> {m. \<forall>m'. (m, m') \<in> beh (lift\<^sub>b (op_vc op v) op (f \<circ> vm_of_ts)) \<longrightarrow> 
                       vm_of_ts m' \<in> Q \<and> ts_is_seq m'}"
     using r by (cases op) (auto elim!: stabilizeE simp: liftg_def wp\<^sub>a.simps)
   show ?case using vc wp by (auto simp: wp_def)
 next
   case gu
   thus ?case using g r apply (cases op) 
-        apply (auto intro!: base_rel_guarI simp: wp\<^sub>a.simps guar_def wp\<^sub>r_def liftg_def split: if_splits)
-       apply force
-    apply force
-     apply force
+        apply (auto intro!: base_rel_guarI id_on_refl simp: wp\<^sub>a.simps guar_def wp\<^sub>r_def liftg_def u_lvarmap split: if_splits)
 
-    sorry
+    using g' 
+    apply auto
+    apply (subgoal_tac "(\<lparr>varmap_st = \<lambda>v. varmap_st (mk_lvarmap (tstack_base x) (vm_of_ts x)) (Gl v),
+                    \<dots> = varmap_rec.more ( (tstack_base x))\<rparr>,
+                 \<lparr>varmap_st =
+                    \<lambda>v. if v = x31 then ev\<^sub>E (varmap_st (mk_lvarmap (tstack_base x) (vm_of_ts x)) \<circ> Ul) x32
+                        else varmap_st (mk_lvarmap (tstack_base x) (vm_of_ts x)) (Gl v),
+                    \<dots> = varmap_rec.more ( (tstack_base x) )\<rparr>)
+                \<in> id_on w (step G)")
+     prefer 2
+    apply blast
+    apply simp
+    apply force_eq
+    apply simp
+    apply force_eq
+    apply force_eq
+    done
+
 next
   case spre
   thus ?case using r by blast
@@ -398,26 +543,44 @@ next
 qed
 
 lemma atomic_spec:
-  assumes r: "reflexive R" "transitive R" "reflexive G"
+  assumes r: "wellformed R G"
+  assumes g: "v\<^sup>U \<subseteq> guar (wp\<^sub>i op o wp\<^sub>a f) (step G)"
+  assumes g': "\<forall>m. v \<subseteq> {s. s \<in> wp\<^sub>i\<^sub>s op {t'. ((gl_restrict s)\<lparr> varmap_rec.more := m \<rparr>, gl_restrict t'\<lparr> varmap_rec.more := m \<rparr>) \<in> id_on w (step G)}}"
   assumes s: "stable\<^sub>L R Q"
   assumes w: "wr op \<subseteq> w" "lk op \<inter> w = {}"
-  shows "R,G \<turnstile>\<^sub>s (stabilize\<^sub>L R (v\<^sup>L \<inter> wp\<^sub>i\<^sub>s op (wp\<^sub>a (f \<circ> ul_restrict) Q))) {Op v op f,r,w} Q"
+  shows "R,G \<turnstile>\<^sub>s (stabilize\<^sub>L R (v \<inter> wp\<^sub>i\<^sub>s op (wp\<^sub>a (f \<circ> ul_restrict) Q))) {Op v op f,r,w} Q"
   unfolding ts_lang_of_vm_lang.simps lift\<^sub>c.simps
 proof (intro basic impI allI conjI atomicI, goal_cases st gu spre spost)
   case st
-  let ?lhs = "spec_pred_of_lvm_pred (stabilize\<^sub>L R (v\<^sup>L \<inter> wp\<^sub>i\<^sub>s op (wp\<^sub>a (f \<circ> ul_restrict) Q))) w"
-  have vc: "?lhs \<subseteq> vc (lift\<^sub>b (ts_pred_of_vm_pred v) op (f \<circ> vm_of_ts))"
+  let ?lhs = "spec_pred_of_lvm_pred (stabilize\<^sub>L R (v \<inter> wp\<^sub>i\<^sub>s op (wp\<^sub>a (f \<circ> ul_restrict) Q))) w"
+  have vc: "?lhs \<subseteq> vc (lift\<^sub>b (op_vc op v) op (f \<circ> vm_of_ts))"
     using r w by (cases op) (auto elim: stabilize\<^sub>LE intro!: spec_ts_mono simp: liftg_def)
-  have wp: "?lhs \<subseteq> {m. \<forall>m'. (m, m') \<in> beh (lift\<^sub>b (ts_pred_of_vm_pred v) op (f \<circ> vm_of_ts)) \<longrightarrow>
-                mk_lvarmap (tstack_base m') (vm_of_ts m') \<in> Q \<and> ts_is_spec m' \<and> w = capped m'}"
+  have wp: "?lhs \<subseteq> {m. \<forall>m'. (m, m') \<in> beh (lift\<^sub>b (op_vc op v) op (f \<circ> vm_of_ts)) \<longrightarrow>
+                mk_lvarmap (tstack_base m') (vm_of_ts m') \<in> Q \<and> ts_is_spec m' \<and> capped m = capped m' \<and> topcapped m = topcapped m'}"
     using r w by (cases op; auto elim!: stabilize\<^sub>LE simp: wp\<^sub>a.simps liftg_def) force_eq+
   show ?case using vc inv wp by (auto simp: wp_def)
 next
   case gu
-  then show ?case using r w apply (cases op) 
-        apply  (auto intro!:  base_rel_guarI simp: wp\<^sub>a.simps guar_def liftg_def wp\<^sub>r_def)
+  thus ?case using g r apply (cases op) 
+        apply (auto intro!: base_rel_guarI id_on_refl simp: wp\<^sub>a.simps guar_def wp\<^sub>r_def liftg_def u_lvarmap split: if_splits)
 
-    sorry (* Problem 2: Need a guarantee / vc combo that works for leak *)
+    using g' 
+    apply auto
+    apply (subgoal_tac "(\<lparr>varmap_st = \<lambda>v. varmap_st (mk_lvarmap (tstack_base x) (vm_of_ts x)) (Gl v),
+                    \<dots> = varmap_rec.more ( (tstack_base x))\<rparr>,
+                 \<lparr>varmap_st =
+                    \<lambda>v. if v = x31 then ev\<^sub>E (varmap_st (mk_lvarmap (tstack_base x) (vm_of_ts x)) \<circ> Ul) x32
+                        else varmap_st (mk_lvarmap (tstack_base x) (vm_of_ts x)) (Gl v),
+                    \<dots> = varmap_rec.more ( (tstack_base x) )\<rparr>)
+                \<in> id_on w (step G)")
+     prefer 2
+    apply blast
+    apply simp
+    apply force_eq
+    apply simp
+    apply force_eq
+    apply force_eq
+    done
 next
   case spre
   thus ?case using r by blast
@@ -429,7 +592,7 @@ qed
 lemma cmp_seq:
   assumes r: "wellformed R G"
   assumes s: "stable\<^sub>t R Q"
-  shows "base_rel_frame_id (step\<^sub>t R),base_rel_guar (step G) w \<turnstile> 
+  shows "base_rel_rely (step\<^sub>t R),base_rel_guar (step G) w \<turnstile> 
           seq_pred_of_vm_pred (stabilize R (wp\<^sub>i (cmp b) Q)) {Basic (liftl (cmp b))} seq_pred_of_vm_pred Q"
   unfolding ts_lang_of_vm_lang.simps lift\<^sub>c.simps liftl_def
 proof (intro basic conjI atomicI, goal_cases st gu  spre spost )
@@ -437,7 +600,7 @@ proof (intro basic conjI atomicI, goal_cases st gu  spre spost )
   thus ?case using r by (auto simp: wp_def elim!: stabilizeE)
 next
   case gu
-  thus ?case using r by (auto intro!: base_rel_guarI  simp: guar_def reflexive_def step_def)
+  thus ?case using r by (auto intro!: base_rel_guarI id_on_refl  simp: guar_def reflexive_def step_def)
 next
   case spre
   thus ?case using r by blast
@@ -449,8 +612,7 @@ qed
 lemma cmp_spec:
   assumes r: "wellformed R G"
   assumes s: "stable\<^sub>L R Q"
-  assumes d: "d > 1"
-  shows "base_rel_frame_id (step\<^sub>t R),base_rel_guar (step G) w \<turnstile> 
+  shows "base_rel_rely (step\<^sub>t R),base_rel_guar (step G) w \<turnstile> 
           spec_pred_of_lvm_pred (stabilize\<^sub>L R (wp\<^sub>i\<^sub>s (cmp b) Q)) w {Basic (liftl (cmp b))} spec_pred_of_lvm_pred Q w"
   unfolding ts_lang_of_vm_lang.simps lift\<^sub>c.simps liftl_def
 proof (intro basic conjI atomicI, goal_cases st gu  spre spost )
@@ -458,7 +620,7 @@ proof (intro basic conjI atomicI, goal_cases st gu  spre spost )
   thus ?case using r by (auto simp: wp_def elim!: stabilize\<^sub>LE)
 next
   case gu
-  thus ?case using r d by (auto intro!: base_rel_guarI  simp: guar_def reflexive_def step_def id_on_def)
+  thus ?case using r by (auto intro!: base_rel_guarI id_on_refl  simp: guar_def reflexive_def step_def )
 next
   case spre
   thus ?case using r by blast
@@ -469,49 +631,38 @@ qed
 
 
 lemma basic_wp:
-  assumes r: "wellformed R G" "reflexive G'"
-  assumes g: "(v \<subseteq> guar (wp\<^sub>i op o wp\<^sub>a f) (step G))"
-  assumes s: "stable (step\<^sub>t R) [Q]\<^sub>;" "stable\<^sub>L R [Q]\<^sub>s"
-  assumes w: "wr op \<subseteq> s" "lk op \<inter> s = {}"
+  assumes r: "wellformed R G" 
+assumes g: "v\<^sup>U \<subseteq> guar (wp\<^sub>i op o wp\<^sub>a f) (step G)"
+  assumes g': "\<forall>m. v \<subseteq> {s. s \<in> wp\<^sub>i\<^sub>s op {t'. ((gl_restrict s)\<lparr> varmap_rec.more := m \<rparr>, gl_restrict t'\<lparr> varmap_rec.more := m \<rparr>) \<in> id_on w (step G)}}"
+assumes s: "stable (step\<^sub>t R) [Q]\<^sub>;" "stable\<^sub>L R [Q]\<^sub>s"
+  assumes w: "wr op \<subseteq> w" "lk op \<inter> w = {}"
 
-  shows "R,G,G' \<turnstile> (wp R (Op v op f) Q) {Op v op f,r,s} Q"
+  shows "R,G \<turnstile> (wp R (Op v op f) Q) {Op v op f,r,w} Q"
 proof ((intro conjI; simp), goal_cases seq spec)
   case seq
-  then show ?case using atomic_seq[OF r(1) g s(1)] by (cases Q, simp)
+  then show ?case using atomic_seq[OF r(1) g g' s(1)] by (cases Q, simp)
 next
   case spec
-  then show ?case using atomic_spec[OF _ _ _ s(2) w] r 
+  then show ?case using atomic_spec[OF r g g' s(2) w] 
     by (cases Q, simp)
 qed
 
 subsection \<open>Frame Reasoning\<close>
 
-lemma base_rel_frame_sz_pushE:
-  assumes "(tstack_push m s, b) \<in> base_rel_frame_sz G (Suc (Suc 0)) w"
-  obtains m' s' where "b = tstack_push m' s'" "(m,m') \<in> base_rel_frame_sz G 1 w"
-  using assms 
-proof -
-  have "tstack_len (tstack_push m s) = tstack_len b" using assms by (auto simp: base_rel_frame_sz_def)
-  hence "tstack_len b \<noteq> 1" by auto
-  then obtain m' s where b: "b = tstack_push m' s" using is_spec_push by blast
-  hence "(m,m') \<in> base_rel_frame_sz G 1 w"
-    using assms unfolding base_rel_frame_sz_def base_rel_def guard_def by auto
-  thus ?thesis using b that by auto
-qed
-
-
 lemma base_rel_guarE:
   assumes "(tstack_push m s, b) \<in> base_rel_guar G w"
-  obtains m' s' where "b = tstack_push m' s'" "(m,m') \<in> base_rel_guar G n"
+  obtains m' s' where "b = tstack_push m' s'" "(m,m') \<in> base_rel_rely (id_on w G)"
   using assms 
 proof -
-  have "tstack_len (tstack_push m s) = tstack_len b" using assms by (auto simp: base_rel_guar_def)
+  have "tstack_len (tstack_push m s) = tstack_len b" using assms base_rel_guar_def 
+    by auto
   hence "tstack_len b \<noteq> 1" by auto
   then obtain m' s where b: "b = tstack_push m' s" using is_spec_push by blast
-  hence "(m,m') \<in> base_rel_guar G n" using assms unfolding base_rel_guar_def base_rel_def by auto
+  hence "(m,m') \<in> base_rel_rely (id_on w G)" using assms 
+    unfolding base_rel_guar_def base_rel_rely_def base_rel_def 
+    by auto
   thus ?thesis using b that by auto
-qed
-
+qed 
 
 lemma mem_restrict:
   assumes "P \<subseteq> P'\<^sup>U"
@@ -530,19 +681,18 @@ text \<open>
 Lower a speculative judgement across the introduction of an empty frame.
 \<close>
 lemma spec_to_seq:
-  assumes "base_rel_frame_id R, base_rel_guar G w \<turnstile> 
+  assumes "base_rel_rely R, base_rel_guar G w \<turnstile> 
             (spec_pred_of_lvm_pred P' w) {r} (spec_pred_of_lvm_pred Q w)"
   assumes "P \<subseteq> P'\<^sup>U"
-  shows "pushrelSame (base_rel_frame_id R),pushrelAll (base_rel_guar G w') \<turnstile> 
+  shows "pushrelSame (base_rel_rely R),pushrelAll (base_rel_rely (id_on w G)) \<turnstile> 
           pushpred (emptyFrame w) (seq_pred_of_vm_pred P) {r} pushpredAll UNIV"
   using assms(1)
 proof (rule conseq, goal_cases pre rely guar post)
   case pre
-  have "\<forall>m. vm_of_ts m \<in> P \<longrightarrow> capped m \<subseteq> w" sorry (* Problem 3: not sure what to do about these sets *)
-  then show ?case unfolding pushpred_def using mem_restrict[OF assms(2)] by force
+  then show ?case unfolding pushpred_def using mem_restrict[OF assms(2)] by auto
 next
   case rely
-  then show ?case unfolding pushrelSame_def base_rel_frame_id_def base_rel_def by auto
+  then show ?case unfolding pushrelSame_def base_rel_rely_def base_rel_def by auto
 next
   case guar
   show ?case by (auto simp: pushrelAll_def elim!: base_rel_guarE) fast
@@ -552,10 +702,10 @@ next
 qed 
 
 lemma spec_to_spec:
-  assumes "base_rel_frame_id R, base_rel_guar G w \<turnstile> 
+  assumes "base_rel_rely R, base_rel_guar G w \<turnstile> 
             (spec_pred_of_lvm_pred P' w) {r} (spec_pred_of_lvm_pred Q w)"
   assumes "P \<subseteq> P'"
-  shows "pushrelSame (base_rel_frame_id R),pushrelAll (base_rel_guar G w) \<turnstile> 
+  shows "pushrelSame (base_rel_rely R),pushrelAll (base_rel_rely (id_on w G)) \<turnstile> 
           pushpred (emptyFrame w) (spec_pred_of_lvm_pred P w) {r} pushpredAll UNIV"
   using assms(1)
 proof (rule conseq, goal_cases pre rely guar post)
@@ -563,702 +713,155 @@ proof (rule conseq, goal_cases pre rely guar post)
   then show ?case unfolding pushpred_def using assms(2) by auto
 next
   case rely
-  then show ?case unfolding pushrelSame_def base_rel_frame_id_def base_rel_def by auto
+  then show ?case unfolding pushrelSame_def base_rel_rely_def base_rel_def by auto
 next
   case guar
-  show ?case apply (auto simp: pushrelAll_def elim!: base_rel_guarE) sorry
+  show ?case by (auto simp: pushrelAll_def elim!: base_rel_guarE) fast
 next
   case post
   then show ?case by (auto intro: is_spec_push simp: pushpredAll_def mk_lvarmap_def)
 qed 
 
-
 lemma stable_conseqI' [intro]:
-  assumes "stable R' P" "Id_on P O R \<subseteq> R'" 
+  assumes "stable R' P" "Id_on P O R \<subseteq> R'"
   shows "stable R P"
   using assms rtrancl_mono unfolding stable_def by blast
 
 lemma spec_judgement:
-  assumes spec: "base_rel_frame_id (step\<^sub>t R),base_rel_guar G' w \<turnstile> spec_pred_of_lvm_pred P' w {r} spec_pred_of_lvm_pred Q' w"
-  assumes wf: "G' \<subseteq> step G \<inter> step\<^sub>t R"
+  assumes spec: "base_rel_rely (step\<^sub>t R),base_rel_guar (step G) w \<turnstile> spec_pred_of_lvm_pred P' w {r} spec_pred_of_lvm_pred Q' w"
+  assumes wf: "id_on w (step G) \<subseteq> step\<^sub>t R" (is "?G \<subseteq> ?R") "id_on w (step G) \<subseteq> step G"
+
   assumes pred: "P \<subseteq> Q" "P \<subseteq> P'\<^sup>U"
   assumes st: "stable\<^sub>t R Q"
 
-  shows "base_rel_frame_id (step\<^sub>t R),base_rel_guar (step G) w \<turnstile> seq_pred_of_vm_pred P {\<triangle> Capture (emptyFrame w) r} seq_pred_of_vm_pred Q"
+  shows "base_rel_rely (step\<^sub>t R),base_rel_guar (step G) w \<turnstile> seq_pred_of_vm_pred P {\<triangle> Capture (emptyFrame w) r} seq_pred_of_vm_pred Q"
 proof -
-  text \<open>Speculative behaviour is stronger than the concrete guarantee\<close>
-  have u: "base_rel_guar G' w \<subseteq> base_rel_guar (step G) w" 
-    using wf by (auto simp: base_rel_guar_def base_rel_def)
 
   text \<open>Speculative behaviour is stronger than the concrete rely, given initial state is not speculative\<close>
-  have m: "\<And>P. Id_on (seq_pred_of_vm_pred P) O base_rel_guar G' w \<subseteq> base_rel_frame_id (step\<^sub>t R)" 
-    using wf by (auto simp: base_rel_guar_def base_rel_def base_rel_frame_id_def)
+  have m: "base_rel_rely ?G \<subseteq> base_rel_rely ?R" 
+    using wf by (auto simp: base_rel_guar_def base_rel_def base_rel_rely_def)
 
-  have st: "stable (base_rel_frame_id (step\<^sub>t R)) (seq_pred_of_vm_pred Q)"
+  have st: "stable (base_rel_rely (step\<^sub>t R)) (seq_pred_of_vm_pred Q)"
     using st by blast
 
-  have "base_rel_frame_id (step\<^sub>t R),base_rel_guar G' w \<turnstile> 
+  have "base_rel_rely (step\<^sub>t R),base_rel_rely ?G \<turnstile> 
       seq_pred_of_vm_pred P {\<triangle> Capture (emptyFrame w) r} seq_pred_of_vm_pred Q"
   proof (rule interr)
     show "seq_pred_of_vm_pred P \<subseteq> seq_pred_of_vm_pred Q" using pred spec_mono by force
   next
-    show "stable (base_rel_frame_id (step\<^sub>t R)) (seq_pred_of_vm_pred Q)" using st by blast
+    show "stable (base_rel_rely (step\<^sub>t R)) (seq_pred_of_vm_pred Q)" using st by blast
   next
-    show "stable (base_rel_guar G' w) (seq_pred_of_vm_pred Q)" using st m
-      by (rule stable_conseqI')
+    show "stable (base_rel_rely ?G) (seq_pred_of_vm_pred Q)" using st m by blast
   next
-    show "base_rel_frame_id (step\<^sub>t R),base_rel_guar G' w \<turnstile> 
+    show "base_rel_rely (step\<^sub>t R),base_rel_rely ?G \<turnstile> 
             seq_pred_of_vm_pred P {Capture (emptyFrame w) r} UNIV" 
       using spec pred(2) by (rule capture[OF spec_to_seq])
   qed
 
-  thus ?thesis using u by blast
+  hence "base_rel_rely (step\<^sub>t R),base_rel_guar (step G) w \<turnstile>
+      seq_pred_of_vm_pred P {\<triangle> Capture (emptyFrame w) r} seq_pred_of_vm_pred Q"
+    apply (rule conseq)
+       apply blast+
+    using wf(2)
+    apply (rule base_rel)
+    apply blast
+    done
+
+  thus ?thesis by blast
 qed
 
 lemma spec_judgement':
-  assumes spec: "base_rel_frame_id (step\<^sub>t R),base_rel_guar G' w \<turnstile> spec_pred_of_lvm_pred P' w {r} spec_pred_of_lvm_pred Q' w"
-  assumes wf: "G' \<subseteq> step G \<inter> step\<^sub>t R"
+  assumes spec: "base_rel_rely (step\<^sub>t R),base_rel_guar (step G) w \<turnstile> spec_pred_of_lvm_pred P' w {r} spec_pred_of_lvm_pred Q' w"
+  assumes wf: "id_on w (step G) \<subseteq> step\<^sub>t R" (is "?G \<subseteq> ?R") "id_on w (step G) \<subseteq> step G"
   assumes pred: "P \<subseteq> Q" "P \<subseteq> P'"
   assumes st: "stable\<^sub>L R Q"
 
-  shows "base_rel_frame_id (step\<^sub>t R),base_rel_guar G' w \<turnstile> spec_pred_of_lvm_pred P w {\<triangle> Capture (emptyFrame w) r} spec_pred_of_lvm_pred Q w"
+  shows "base_rel_rely (step\<^sub>t R),base_rel_guar (step G) w \<turnstile> spec_pred_of_lvm_pred P w {\<triangle> Capture (emptyFrame w) r} spec_pred_of_lvm_pred Q w"
 proof -
-  text \<open>Speculative behaviour is stronger than the concrete guarantee\<close>
-  have u: "base_rel_guar G' w \<subseteq> base_rel_guar (step G) w" 
-    using wf by (auto simp: base_rel_guar_def base_rel_def)
-
   text \<open>Speculative behaviour is stronger than the concrete rely, given initial state is not speculative\<close>
-  have m: "\<And>P. Id_on (spec_pred_of_lvm_pred P w) O base_rel_guar G' w \<subseteq> base_rel_frame_id (step\<^sub>t R)" 
-    using wf apply (auto simp: base_rel_guar_def base_rel_def base_rel_frame_id_def)
-    sorry
+  have m: "base_rel_rely ?G \<subseteq> base_rel_rely ?R" 
+    using wf by (auto simp: base_rel_guar_def base_rel_def base_rel_rely_def)
 
-  have st: "stable (base_rel_frame_id (step\<^sub>t R)) (spec_pred_of_lvm_pred Q w)"
+  have st: "stable (base_rel_rely (step\<^sub>t R)) (spec_pred_of_lvm_pred Q w)"
     using st by blast
 
-  have "base_rel_frame_id (step\<^sub>t R),base_rel_guar G' w \<turnstile> 
+  have "base_rel_rely (step\<^sub>t R),base_rel_rely ?G \<turnstile> 
       spec_pred_of_lvm_pred P w {\<triangle> Capture (emptyFrame w) r} spec_pred_of_lvm_pred Q w"
   proof (rule interr)
     show "spec_pred_of_lvm_pred P w \<subseteq> spec_pred_of_lvm_pred Q w" using pred spec_mono by force
   next
-    show "stable (base_rel_frame_id (step\<^sub>t R)) (spec_pred_of_lvm_pred Q w)" using st by blast
+    show "stable (base_rel_rely (step\<^sub>t R)) (spec_pred_of_lvm_pred Q w)" using st by blast
   next
-    show "stable (base_rel_guar G' w) (spec_pred_of_lvm_pred Q w)" using st m sorry
+    show "stable (base_rel_rely ?G) (spec_pred_of_lvm_pred Q w)" using st m by blast
   next
-    show "base_rel_frame_id (step\<^sub>t R),base_rel_guar G' w \<turnstile> 
+    show "base_rel_rely (step\<^sub>t R),base_rel_rely ?G \<turnstile> 
             spec_pred_of_lvm_pred P w {Capture (emptyFrame w) r} UNIV" 
       using spec pred(2) by (rule capture[OF spec_to_spec])
   qed
 
-  thus ?thesis using u by auto
-qed
-
-(*
-
-definition stabilize\<^sub>s where 
-  "stabilize\<^sub>s R P \<equiv> {m. \<forall>m'. (glb (gl_restrict m),glb m') \<in> R \<longrightarrow> rg (gl_restrict m) = rg m' \<longrightarrow> m' \<in> [P]\<^sub>;}"
-
-
-(*
-lemma vm_of_ts_wp:
-  assumes "vm_of_ts x \<in> c \<inter> wp\<^sub>i \<alpha> (wp\<^sub>a f Q)"
-  shows "x \<in> State.wp (ts_pred_of_vm_pred c) (st_beh\<^sub>i \<alpha> O {(t, t'). t' = tauxupd t (f \<circ> vm_of_ts)}) (ts_pred_of_vm_pred Q)"
-proof -
-  have x[intro]: "vm_of_ts x \<in> c" "vm_of_ts x \<in> wp\<^sub>i \<alpha> (wp\<^sub>a f Q)" using assms by auto
-  note wp_def[simp] ts_pred_of_vm_pred_def[simp]
-
-  show ?thesis using x
-  proof (cases \<alpha>)
-    case (assign v val)
-    then show ?thesis
-    using x vm_of_ts_bothupd[where ?s=x and ?v=v]
-    by (auto simp add: vm_of_ts_auxupd vm_of_ts.rep_eq)
-  next
-    case (cmp x2)
-    then show ?thesis  
-    using x
-    by (auto simp add: vm_of_ts_auxupd, simp add: vm_of_ts.rep_eq)
-  next
-    case (leak v val)
-    then show ?thesis 
-    using x vm_of_ts_bothupd[where ?s=x and ?v=v]
-    by (auto simp add: vm_of_ts_auxupd vm_of_ts.rep_eq)
-  qed (simp_all add: vm_of_ts_auxupd)
-qed *)
-
-lemma wp_of_liftg:
-  "\<And>x. reflexive R \<Longrightarrow> vm_of_ts x \<in> stabilize R ((vm_of_ts ` c)\<^sup>L \<inter> wp\<^sub>i\<^sub>s \<alpha> {t. t\<lparr>varmap_rec.more := f (ts_of_vm t)\<rparr> \<in> (Q\<^sup>G)\<^sup>U}\<^sup>L)\<^sup>U \<Longrightarrow> x \<in> wp\<^sub>\<alpha> (liftg c \<alpha> f) (ts_pred_of_vm_pred Q)" 
-unfolding liftg_def apply simp
-proof goal_cases
-  case (1 x)
-  have "vm_of_ts x \<in> ((vm_of_ts ` c)\<^sup>L \<inter> wp\<^sub>i\<^sub>s \<alpha> {t. t\<lparr>varmap_rec.more := f (ts_of_vm t)\<rparr> \<in> (Q\<^sup>G)\<^sup>U}\<^sup>L)\<^sup>U"
-    using "local.1"(1) "local.1"(2) wp.stabilizeE sorry
-  then show ?case unfolding wp_def stabilize_def sorry
-qed
-
-lemma vm_of_ts_wp_liftg:
-  "\<And>x. vm_of_ts x \<in> c \<inter> wp\<^sub>i \<alpha> (wp\<^sub>a f Q) \<Longrightarrow> x \<in> wp\<^sub>\<alpha> (liftg (ts_pred_of_vm_pred c) \<alpha> (f \<circ> vm_of_ts)) (ts_pred_of_vm_pred Q)" 
-unfolding liftg_def 
-by (simp add: ts_pred_of_vm_pred.transfer vm_of_ts_wp)
-
-(*
-lemma guar_of_liftg:
-  assumes "c \<subseteq> local.guar (wp\<^sub>i \<alpha> \<circ> wp\<^sub>a f) (step G)"
-  shows "guar\<^sub>\<alpha> (liftg (ts_pred_of_vm_pred c) \<alpha> (f \<circ> vm_of_ts)) (ts_rel_of_vm_rel (step G))"
-using assms 
-unfolding liftg_def guar_def ts_pred_of_vm_pred_def ts_rel_of_vm_rel_def
-proof (clarsimp, goal_cases)
-  case (1 x y)
-  hence x: "vm_of_ts x \<in> wp\<^sub>i \<alpha> {ta. (vm_of_ts x, ta\<lparr>varmap_rec.more := f ta\<rparr>) \<in> step G}"
-    unfolding wp\<^sub>r_def by auto
-  then show ?case using 1
-  proof (cases \<alpha>)
-    case (assign v val)
-    then show ?thesis using x 1 vm_of_ts_bothupd[where ?s=x and ?v=v]
-    by (simp add: vm_of_ts.rep_eq)    
-  next
-    case (cmp _)
-    then show ?thesis using x 1 vm_of_ts_auxupd[of f x]
-    by (clarsimp simp add: vm_of_ts.rep_eq)
-  next
-    case (leak v val)
-    then show ?thesis using x 1 vm_of_ts_bothupd[where ?s=x and ?v=v] 
-    by (simp add: vm_of_ts.rep_eq)
-  qed (auto simp add: vm_of_ts_auxupd)
-qed *)
-
-lemma guar_of_liftg':
-  assumes "c \<subseteq> guar (wp\<^sub>i \<alpha> \<circ> wp\<^sub>a f) (step G)" 
-  shows "State.guar {s. vm_of_ts s \<in> c \<and> ts_is_seq s} {(s, s'). (s, s') \<in> st_beh\<^sub>i \<alpha> O {(t, t'). t' = tauxupd t (f \<circ> vm_of_ts)} \<and> ts_is_seq s \<and> ts_is_seq s'} (seq_rel_of_vm_rel (step G))"
-proof (cases \<alpha>)
-  case (assign x11 x12)
-  then show ?thesis apply simp unfolding liftg_def seq_rel_of_vm_rel_def ts_pred_of_vm_pred_def guar_def apply auto
-    unfolding ts_rel_of_vm_rel_def
-     apply auto using assms
-     sorry
-next
-  case (cmp x2)
-  then show ?thesis sorry
-next
-  case (leak x31 x32)
-  then show ?thesis sorry
-next
-  case full_fence
-  then show ?thesis sorry
-next
-  case nop
-  then show ?thesis sorry
-qed
-
-lemma stable_ts_rel_from_stablet [elim]: 
-  assumes "stable\<^sub>t R P"
-  shows "State.stable (ts_rel_of_vm_rel (step\<^sub>t R)) (ts_pred_of_vm_pred (P))"
-using assms 
-unfolding stable_def stabilize_def ts_pred_of_vm_pred_def ts_rel_of_vm_rel_def step\<^sub>t_def transitive_def
-by auto
-
-lemma stable_seq_from_stable_ts:
-  assumes "State.stable (ts_rel_of_vm_rel (step\<^sub>t R)) (ts_pred_of_vm_pred Q)"
-  shows "State.stable (seq_rel_of_vm_rel (step\<^sub>t R)) (seq_pred_of_vm_pred Q)"
-using assms
-unfolding stable_def seq_pred_of_vm_pred_def seq_rel_of_vm_rel_def
-using ts_upper_of_seq 
-by clarsimp fastforce
-
-lemma stable_seq_rel_from_stablet [intro]:
-  assumes "stable\<^sub>t R Q"
-  shows "State.stable (seq_rel_of_vm_rel (step\<^sub>t R)) (seq_pred_of_vm_pred Q)"
-using assms stable_seq_from_stable_ts stable_ts_rel_from_stablet by auto
-
-
-(* lemma stept_stept [simp]: "step\<^sub>t (step\<^sub>t G) = step\<^sub>t G"  *)
-(* unfolding step\<^sub>t_def by simp *)
-
-(* lemma step_step [simp]: "step (step G) = step G"  *)
-(* unfolding step_def by simp *)
-
-lemma tauxupd_more [simp]: "{(t, t'). t' = tauxupd t (varmap_rec.more \<circ> vm_of_ts)} = Id" 
-unfolding tauxupd_def auxupd_def vm_of_ts_def 
-by (auto simp add: Rep_tstackI(1) Rep_tstack_inverse)
-
-lemma wp\<^sub>a_more [simp]: "wp\<^sub>a varmap_rec.more = id" 
-by standard (simp add: wp.wp\<^sub>a.simps)
-
-lemma [simp]: "(\<lambda>s. frame.more (last (Rep_tstack s))) = (\<lambda>s. varmap_rec.more (vm_of_ts s))" 
-proof
-  show "\<And>s. frame.more (last (Rep_tstack s)) = varmap_rec.more (vm_of_ts s)"
-  unfolding vm_of_ts_def by auto
-qed
-
-lemma [simp]: "ts_pred_of_vm_pred UNIV = UNIV"
-unfolding ts_pred_of_vm_pred_def by simp
-
-section \<open>Soundness\<close>
-
-
-lemma h2: 
-  assumes "(s,s') \<in> beh\<^sub>a auxop"
-  shows "tstack_len s = tstack_len s'"
-  sorry
-
-lemma h1:
-  assumes "P \<subseteq>\<^sub>s (stabilize\<^sub>L R (c\<^sup>L \<inter> wp\<^sub>i\<^sub>s \<alpha> (wp\<^sub>a (f \<circ> gl_restrict) [Q]\<^sub>s)), 
-                                stabilize R (c \<inter> wp\<^sub>i \<alpha> (wp\<^sub>a f [Q]\<^sub>;)))"
-          "wellformed R G" "stable\<^sub>t R [Q]\<^sub>;" 
-  assumes "vm_of_ts x \<in> [P]\<^sub>;"
-  shows "x \<in> State.wp {s. vm_of_ts s \<in> c \<and> ts_is_seq s} {(s, s'). (s, s') \<in> st_beh\<^sub>i \<alpha> O {(t, t'). t' = tauxupd t (f \<circ> vm_of_ts)} \<and> ts_is_seq s \<and> ts_is_seq s'} (seq_pred_of_vm_pred [Q]\<^sub>;)"
-sorry 
-
-  
-lemma conseq_s:
-  assumes "R,G \<turnstile>\<^sub>s P {op} Q"
-  assumes "P' \<subseteq>\<^sub>s P"
-  shows "R,G \<turnstile>\<^sub>s P' {op} Q"
-  using assms seq_pred_of_vm_pred_subset 
-  apply auto
-  apply (rule conseq)
-  apply simp_all
-  apply (intro spec_pred_of_lvm_pred_subset seq_pred_of_vm_pred_subset)
-  by auto
-
-(*
-lemma h3:
-  "ts_is_seq x \<Longrightarrow> vm_of_ts x \<in> wp\<^sub>a f Q \<Longrightarrow> tauxupd x (f \<circ> vm_of_ts) \<in> seq_pred_of_vm_pred Q"
-  unfolding seq_pred_of_vm_pred_def
-  by (simp add: vm_of_ts_auxupd wp.wp\<^sub>a.simps ts_is_seq_def, insert tauxupd_len[of x], simp)
-
-lemma basic_wp\<^sub>i_1_assign:
-  fixes xa x11 x12 f
-  defines "rhs \<equiv> (tauxupd (tupdate xa x11 (ev\<^sub>E (tlookup xa) x12)) (f \<circ> vm_of_ts))"
-  assumes "vm_of_ts xa\<lparr>varmap_st := (varmap_st (vm_of_ts xa))(x11 := ev\<^sub>E (varmap_st (vm_of_ts xa)) x12)\<rparr> \<in> wp\<^sub>a f Qseq"
-  assumes "ts_is_seq xa"
-  shows 
-    "rhs \<in> seq_pred_of_vm_pred Qseq"
-    "ts_is_seq rhs"
-proof -
-  show "rhs \<in> seq_pred_of_vm_pred Qseq"
-    unfolding rhs_def
-    using assms(2) unfolding wp\<^sub>a.simps seq_pred_of_vm_pred_def
-    apply auto 
-    apply (metis varmap_rec.select_convs(1) vm_of_ts.abs_eq vm_of_ts_bothupd)
-    by (metis assms(3) tauxupd_len ts_is_seq_def tupdate_len)
-  show "ts_is_seq rhs"
-    unfolding rhs_def using assms(3) unfolding ts_is_seq_def using tupdate_len tauxupd_len by metis
-qed *)
-
-lemma basic_wp\<^sub>i_1_assign_spec:
-  assumes "\<alpha> = assign x11 x12"
-  assumes "ts_is_spec x"
-  assumes "x \<in> spec_pred_of_lvm_pred (wp\<^sub>i\<^sub>s \<alpha> (wp\<^sub>a (f \<circ> gl_restrict) Qspec))"
-  shows "tauxupd (tupdate x x11 (ev\<^sub>E (tlookup x) x12)) (f \<circ> vm_of_ts) \<in> spec_pred_of_lvm_pred Qspec" (is "?ts \<in> \<dots>")
-    "ts_is_spec (tauxupd (tupdate x x11 (ev\<^sub>E (tlookup x) x12)) (f \<circ> vm_of_ts))"
-using assms
-unfolding spec_pred_of_lvm_pred_def
-proof (clarsimp simp add: id_def, goal_cases)
-  case (1 v)
-  let ?v_ = "v\<lparr>varmap_st := (varmap_st v)(Ul x11 := ev\<^sub>E (varmap_st v) (map\<^sub>E Ul id id x12))\<rparr>"
-  let ?v = "?v_\<lparr>varmap_rec.more := f (gl_restrict ?v_)\<rparr>"
-
-  have tlookup: "tlookup x va = varmap_st v (Ul va)" for va
-    using 1(4) unfolding tlookup_def vm_of_ts_def by auto
-
-  have ev: "ev\<^sub>E (tlookup x) xa = (ev\<^sub>E (varmap_st v) \<circ> map\<^sub>E Ul id id) xa" for xa
-  by (induct xa, simp_all add: tlookup id_def comp_def) (metis (mono_tags, lifting) map_eq_conv)
-
-  have "ev\<^sub>E (\<lambda>va. varmap_st v (Ul va)) x12 = ev\<^sub>E (tlookup x) x12"
-    using tlookup by presburger
-
-  have notnone: "frame_st (last (Rep_tstack (tauxupd (tupdate x x11 (ev\<^sub>E (tlookup x) x12)) (\<lambda>x. f (vm_of_ts x))))) va \<noteq> None" for va
-    by blast
-
-    
-  show ?case
-  proof (standard, intro conjI)
-    show "?v \<in> Qspec" using 1(2) by (cases x12) (auto simp add: id_def wp\<^sub>a.simps)
-    show "ts_is_spec (tauxupd (tupdate x x11 (ev\<^sub>E (tlookup x) x12)) (f \<circ> vm_of_ts))" using 1(2,3) by clarify (metis tauxupd_len ts_is_seq_def tupdate_len)
-    show "vm_of_ts ?ts = \<lparr>varmap_st = \<lambda>va. varmap_st (?v) (Ul va), \<dots> = varmap_rec.more (?v)\<rparr>" unfolding vm_of_ts_def apply auto apply standard apply (case_tac "va = x11") apply auto apply (cases x12) apply auto using 1(4)
-    apply (simp add: vm_of_ts.abs_eq) apply (subgoal_tac "ev\<^sub>E (tlookup x) = (ev\<^sub>E (varmap_st v) \<circ> map\<^sub>E Ul id id)") apply auto apply standard  
-    using ev apply blast 
-    apply (simp add: tlookup)  apply (rule arg_cong[where ?f=f]) apply auto apply standard apply (case_tac "x11 = xa") apply auto using 1(4) unfolding vm_of_ts_def apply auto 
-    sorry (* we need properties constraining the acceptable auxfns (i.e. they are minimally state-dependent). or, we need to ignore them. *)
-    show "tstack_base ?ts = \<lparr>varmap_st = \<lambda>va. varmap_st (?v) (Gl va), \<dots> = varmap_rec.more (?v)\<rparr>" unfolding tstack_base_def apply auto apply standard unfolding comp_def using notnone sorry
-  qed
-next
-  case 2
-  show ?case using assms(2) tauxupd_len tupdate_len ts_is_seq_def by metis
-qed
-
- *)
-
-
-(*
-
-text \<open>Basic Rule for operations with vc c\<close>
-lemma basic_wp\<^sub>i_1:
-  assumes "P \<subseteq>\<^sub>s (stabilize\<^sub>L R (c\<^sup>L \<inter> wp\<^sub>i\<^sub>s \<alpha> (wp\<^sub>a (f \<circ> gl_restrict) [Q]\<^sub>s)), 
-                 stabilize R (c \<inter> wp\<^sub>i \<alpha> (wp\<^sub>a f [Q]\<^sub>;)))"
-          "wellformed R G" "stable\<^sub>t R [Q]\<^sub>;" 
-  assumes "c \<subseteq> guar (wp\<^sub>i \<alpha> o wp\<^sub>a f) (step G)"
-  shows "R,G \<turnstile>\<^sub>s P {Op (ts_pred_of_vm_pred c) \<alpha> (f \<circ> vm_of_ts)} Q"
-proof -
-  let ?P = "(stabilize\<^sub>L R (c\<^sup>L \<inter> wp\<^sub>i\<^sub>s \<alpha> (wp\<^sub>a (f \<circ> gl_restrict) [Q]\<^sub>s)), 
-                 stabilize R (c \<inter> wp\<^sub>i \<alpha> (wp\<^sub>a f [Q]\<^sub>;)))"
-  have "R,G \<turnstile>\<^sub>s ?P {Op (ts_pred_of_vm_pred c) \<alpha> (f \<circ> vm_of_ts)} Q"
-  proof (standard, goal_cases nonspec spec)
-    case nonspec
-    obtain a v b where ba: "Basic (a, v, b) = nonspec (lift\<^sub>c (Op (ts_pred_of_vm_pred c) \<alpha> (f \<circ> vm_of_ts)) com.Nil {})" 
-      by (simp add: liftg_def)
-    have a: "a = (\<alpha>, (f \<circ> vm_of_ts))" using ba by (simp add: liftg_def)
-    have v: "v = {x \<in> (ts_pred_of_vm_pred c). ts_is_seq x}" using ba by (simp add: liftg_def)
-    have b: "b = beh\<^sub>a (\<alpha>, f \<circ> vm_of_ts)" using ba by (simp add: liftg_def)
-    have refl: "reflexive R" using assms(2) by simp
-    have stabilizeE': "x \<in> X" if "x \<in> stabilize R X" for x X using refl stabilizeE that by auto
-    show ?case unfolding b ba[symmetric] apply (intro basic) unfolding atomic_rule_def a v b
-    proof (simp only: seq_part.simps, intro conjI impI, goal_cases)
-      case 1
-      then show ?case
-      proof standard
-        fix x
-        assume x: "x \<in> seq_pred_of_vm_pred (stabilize R (c \<inter> wp\<^sub>i \<alpha> (wp\<^sub>a f [Q]\<^sub>;)))"
-        hence lhs: "x \<in> seq_pred_of_vm_pred (c \<inter> wp\<^sub>i \<alpha> (wp\<^sub>a f [Q]\<^sub>;))" 
-          using stabilizeE' seq_pred_of_vm_pred_subset by blast
-        have x1: "vm_of_ts x \<in> c" "ts_is_seq x"
-          using lhs unfolding seq_pred_of_vm_pred_def by (simp, simp)
-        have x2: "vm_of_ts x \<in> wp\<^sub>i \<alpha> (wp\<^sub>a f [Q]\<^sub>;)" 
-          using lhs unfolding seq_pred_of_vm_pred_def by simp
-        note xx = x1 x2
-        thus rhs: "x \<in> wp\<^sub>\<alpha> ((\<alpha>, f \<circ> vm_of_ts), {x \<in> ts_pred_of_vm_pred c. ts_is_seq x}, beh\<^sub>a (\<alpha>, f \<circ> vm_of_ts)) (seq_pred_of_vm_pred [Q]\<^sub>;)"
-        proof (cases \<alpha>)
-          case (assign x11 x12)
-          thus ?thesis unfolding wp_def apply (auto simp add: xx) apply (rule basic_wp\<^sub>i_1_assign)
-          using assign xx by auto
-        next
-          case (cmp x2)
-          thus ?thesis unfolding wp_def apply (auto simp add: xx) using xx unfolding cmp 
-          apply auto
-          apply (simp add: vm_of_ts.abs_eq)
-          using h3 by auto
-        next
-          case (leak x31 x32)
-          thus ?thesis unfolding wp_def apply (auto simp add: xx) apply (rule basic_wp\<^sub>i_1_assign)
-          using leak xx by auto
-        next
-          case full_fence
-          thus ?thesis unfolding wp_def apply (auto simp add: xx) 
-          using h3 x2 xx(2) by auto
-        next
-          case nop
-          then show ?thesis unfolding nop 
-            apply auto unfolding wp_def apply (auto simp add: xx)
-            using x2 unfolding nop by (auto simp add: h3 xx(2))
-        qed
-      qed
-    next
-      case 2
-      then show ?case apply (clarsimp, intro conjI) using stabilizeE' unfolding seq_pred_of_vm_pred_def by auto 
-    next
-      case 3
-      have q: "seq_pred_of_vm_pred ((c \<inter> wp\<^sub>i \<alpha> (wp\<^sub>a f [Q]\<^sub>;))) \<subseteq>  {x \<in> ts_pred_of_vm_pred c. ts_is_seq x}" 
-        apply (clarsimp, intro conjI) using stabilizeE' unfolding seq_pred_of_vm_pred_def by auto
-      then show ?case unfolding seq_rel_of_vm_rel_def seq_pred_of_vm_pred_def apply auto 
-      proof goal_cases
-        case 1
-        have l: "\<And>x. ts_is_seq x \<Longrightarrow>  butlast (Rep_tstack x) = []" unfolding ts_is_seq_def tstack_len_def
-          by (simp add: butlast_conv_take)
-        have c: "c \<subseteq> local.guar (wp\<^sub>i \<alpha> \<circ> wp\<^sub>a f) (step G)" using assms by simp
-        hence vm_of_ts_c: "\<And>x. vm_of_ts x \<in> c \<Longrightarrow> vm_of_ts x  \<in> (local.guar (wp\<^sub>i \<alpha> \<circ> wp\<^sub>a f) (step G))" by auto
-        show ?case unfolding guar_def apply auto defer unfolding ts_is_seq_def tstack_upper_def using tstack_len_of_st_beh  apply simp
-        apply (metis One_nat_def l tauxupd_len ts_is_seq_def)
-        using q
-        proof goal_cases
-          case (1 x y)
-            note c2 = vm_of_ts_c[OF 1(1)]
-            have "(vm_of_ts x, vm_of_ts (tauxupd y (f \<circ> vm_of_ts))) \<in> ((step G))" using vm_of_ts_c[OF 1(1)] unfolding wp\<^sub>r_def apply auto
-            proof (cases \<alpha>)
-              case (assign x11 x12)
-              have y: "tupdate x x11 (ev\<^sub>E (tlookup x) x12) = y" using 1(3) unfolding assign by auto
-              show ?thesis using c2 unfolding wp\<^sub>r_def unfolding wp\<^sub>a.simps y apply (auto simp add: assign) by (metis varmap_rec.select_convs(1) vm_of_ts.abs_eq vm_of_ts_bothupd y) 
-            next
-              case (cmp x2)
-              then show ?thesis using c2 1(3) unfolding wp\<^sub>r_def cmp apply (auto) apply (simp add: vm_of_ts.abs_eq) by (simp add: vm_of_ts_auxupd wp.wp\<^sub>a.simps)
-            next
-              case (leak x31 x32)
-              then show ?thesis using c2 1(3) unfolding wp\<^sub>r_def leak wp\<^sub>a.simps apply auto by (metis varmap_rec.select_convs(1) vm_of_ts.abs_eq vm_of_ts_bothupd) 
-            next
-              case full_fence
-              then show ?thesis using c2 1(3) unfolding wp\<^sub>r_def full_fence wp\<^sub>a.simps apply auto by (simp add: vm_of_ts_auxupd)
-            next
-              case nop
-              then show ?thesis using c2 1(3) unfolding wp\<^sub>r_def nop wp\<^sub>a.simps apply simp by (simp add: vm_of_ts_auxupd)
-            qed
-          then show ?case using ts_rel_of_vm_rel_from_vm_of_ts by auto
-        qed
-      qed 
-    next
-      case 4
-      then show ?case using assms by auto
-    next
-      case 5
-      then show ?case using assms stable_ts_rel_from_stablet[OF assms(3)] by auto
-    qed
-  next
-    case spec
-    show ?case
-    unfolding liftg_def
-    proof (simp, intro basic, simp only: atomic_rule_def, intro conjI impI subsetI, goal_cases)
-      case (1 x)
-      thm assms
-      have x: "x \<in> spec_pred_of_lvm_pred ((c\<^sup>L \<inter> wp\<^sub>i\<^sub>s \<alpha> (wp\<^sub>a (f \<circ> gl_restrict) [Q]\<^sub>s)))" using 1 assms(2) by auto
-      have x_in_c: "x \<in> spec_pred_of_lvm_pred c\<^sup>L" using  x spec_pred_of_lvm_pred_subset by blast
-      have x_in_wp: "x \<in> spec_pred_of_lvm_pred (wp\<^sub>i\<^sub>s \<alpha> (wp\<^sub>a (f \<circ> gl_restrict) [Q]\<^sub>s))" using  x spec_pred_of_lvm_pred_subset by blast
-      have vm_x_in_c: "vm_of_ts x \<in> c" using x_in_c unfolding ul_lift_pred_def spec_pred_of_lvm_pred_def by auto
-      have "x \<in> vc (liftg (ts_pred_of_vm_pred c) \<alpha> (f \<circ> vm_of_ts))" using assms(4) x_in_c vm_x_in_c by (simp add: liftg_def)
-
-      then show ?case apply (cases \<alpha>) apply auto unfolding wp_def apply auto unfolding liftg_def apply auto using   x_in_wp  apply auto unfolding wp\<^sub>a.simps apply auto sorry
-    next
-      case (2 x)
-      then show ?case sorry
-    next
-      case 3
-      then show ?case sorry
-    next
-      case 4
-      then show ?case sorry
-    next
-      case 5
-      then show ?case sorry
-      qed
-  qed                 
-  thus ?thesis using conseq_s assms(1) by blast
-qed
-
-text \<open>Basic Rule for operations without vc\<close>
-lemma basic_wp\<^sub>i_2:
-  assumes "P \<subseteq>\<^sub>s (stabilize\<^sub>L R (wp\<^sub>i\<^sub>s \<alpha>[Q]\<^sub>s), stabilize R (wp\<^sub>i \<alpha> [Q]\<^sub>;))"
-          "wellformed R G" "stable\<^sub>t R [Q]\<^sub>;" 
-  assumes "\<forall>m. m \<in> guar (wp\<^sub>i \<alpha>) (step G)"
-  shows "R,G \<turnstile>\<^sub>s P {Op UNIV \<alpha> taux} Q"
-  sorry (*
-proof -
-  have x: "vm_of_ts x \<in> wp\<^sub>i \<alpha> Q" if "x \<in> ts_pred_of_vm_pred (stabilize R (wp\<^sub>i \<alpha> Q))" for x 
-    using assms(1,2) stabilizeE using that vm_of_ts_in_ts_pred_of_vm_pred by blast
-  have 1: "ts_rel_of_vm_rel (step\<^sub>t R),ts_rel_of_vm_rel(step G) \<turnstile>\<^sub>A ts_pred_of_vm_pred(stabilize R (wp\<^sub>i \<alpha> Q)) {(liftg UNIV \<alpha> taux)} ts_pred_of_vm_pred Q"
-  proof (rule atomicI, goal_cases)
-    case 1
-    have "x \<in> wp\<^sub>\<alpha> (liftg UNIV \<alpha> taux) (ts_pred_of_vm_pred Q)" if "x \<in> ts_pred_of_vm_pred (stabilize R (wp\<^sub>i \<alpha> Q))" for x
-    using x[of x, OF that] vm_of_ts_wp_liftg[where ?c = UNIV and ?f = varmap_rec.more] 
-    unfolding liftg_def wp_def by simp
-    thus ?case by auto
-  next
-    case 2
-    hence univ: "UNIV \<subseteq> local.guar (wp\<^sub>i \<alpha> \<circ> wp\<^sub>a varmap_rec.more) (step G)" using assms(4) by auto
-    have "guar\<^sub>\<alpha> (liftg (ts_pred_of_vm_pred UNIV) \<alpha> taux) (ts_rel_of_vm_rel (step G))"
-    using guar_of_liftg[where ?c = UNIV and ?f = varmap_rec.more, OF univ]
-    unfolding taux_def comp_def by auto
-    then show ?case by simp 
-  next
-    case 3
-    then show ?case using assms(2) by auto
-  next
-    case 4
-    then show ?case using assms(3) by auto
-  qed
-  then have "R,G \<turnstile>\<^sub>s stabilize R (wp\<^sub>i \<alpha> Q) {Op UNIV \<alpha> taux} Q"
-    by simp (rule rules.basic)
-  thus ?thesis using assms(1) conseq 
-  by (simp add: ts_pred_of_vm_pred.rep_eq vimage_mono)
-qed
-  oops *)
-
-lemma lift_wp:
-  assumes "P \<subseteq> wp\<^sub>\<alpha> (c,vm_pred_of_ts_pred V,vm_rel_of_ts_rel (beh\<^sub>a R)) Q"
-  shows "seq_pred_of_vm_pred P \<subseteq> wp\<^sub>\<alpha> (c,V,beh\<^sub>a R) (seq_pred_of_vm_pred Q)"
-  using assms unfolding seq_pred_of_vm_pred_def wp_def vm_pred_of_ts_pred_def vm_rel_of_ts_rel_def
-  apply auto
-  sorry
-
-text \<open>A rule for cmp operations, used for If/While\<close>
-lemma cmp_sound [intro!]:
-  assumes "wellformed R G" "stable\<^sub>t R [Q]\<^sub>;"
-  assumes "P \<subseteq>\<^sub>s (stabilize\<^sub>L R (wp\<^sub>i\<^sub>s (cmp b) [Q]\<^sub>s), stabilize R (wp\<^sub>i (cmp b) [Q]\<^sub>;))" (is "P \<subseteq>\<^sub>s ?P")
-  shows "R,G \<turnstile>\<^sub>s P {Op UNIV (cmp b) varmap_rec.more} Q"
-proof -
-  have "R,G \<turnstile>\<^sub>s ?P {Op UNIV (cmp b) varmap_rec.more} Q"
-  proof (intro conjI, goal_cases seq spec)
-    case seq
-
-    then show ?case
-      apply (simp add: liftg_def del: beh\<^sub>a.simps)
-      apply (rule basic)
-      apply (rule atomicI)
-      apply (rule lift_wp)
-
-      apply auto
-
-      apply (auto simp: wp_def liftg_def guar_def)[2]
-
-    sorry
-next
-  case spec
-  then show ?case sorry
-qed
-  
-
-subsection \<open>State Ordering\<close>
-
-text \<open>Properties of the state ordering. Essentially entailment with preservation of stability\<close>
-
-text \<open>The ordering is reflexive\<close>
-lemma refl_ord:
-  "R,G \<turnstile>\<^sub>w P \<ge> P"
-  unfolding context_order_def by (auto simp: )
-
-text \<open>It is possible to strengthen the RHS\<close>
-lemma assert_ord:
-  "R,G \<turnstile>\<^sub>w P \<inter> assert A \<ge> P"
-  by (cases A) (auto simp: context_order_def assert_def) 
-
-text \<open>Stabilize Ordering\<close>
-lemma stabilize_ord [intro]:
-  assumes "P \<subseteq> Q"
-  shows "R,G \<turnstile>\<^sub>w stabilize R P \<ge> Q"
-  using assms stabilizeE unfolding context_order_def 
-  by blast
-
-subsection \<open>Rules\<close>
-
-text \<open>If Rule\<close>
-
-lemma if_wp:
-  "R,G \<turnstile>\<^sub>w P\<^sub>1 {c\<^sub>1} Q \<Longrightarrow> R,G \<turnstile>\<^sub>w P\<^sub>2 {c\<^sub>2} Q \<Longrightarrow>
-  R,G \<turnstile>\<^sub>w stabilize R ((wp\<^sub>s (vm_lang_of_ts_lang (If b c\<^sub>1 c\<^sub>2)) (Q\<^sup>G))\<^sup>U) {If b c\<^sub>1 c\<^sub>2} UNIV \<Longrightarrow>
-  P \<subseteq> (wp\<^sub>i (cmp b) P\<^sub>1 \<inter> wp\<^sub>i (ncmp b) P\<^sub>2) \<Longrightarrow>
-            R,G \<turnstile>\<^sub>w stabilize R P {If b c\<^sub>1 c\<^sub>2} Q"
-  unfolding valid_def 
-sorry
-
-text \<open>While Rule\<close>
-lemma while_wp:
-  assumes "R,G \<turnstile>\<^sub>w P {c} stabilize R J" (is "R,G \<turnstile>\<^sub>w P {c} ?I")
-  assumes "J \<subseteq> (wp\<^sub>i (cmp b) P \<inter> wp\<^sub>i (ncmp b) Q)"
-  shows "R,G \<turnstile>\<^sub>w ?I {While b Imix Ispec c} Q"
-  unfolding valid_def lift\<^sub>c.simps
-proof (intro impI conjI rules.choice rules.seq)
-  assume "wellformed R G \<and> stable\<^sub>t R Q \<and> guar\<^sub>c (While b Imix Ispec c) (G)"
-  thus "step\<^sub>t R,step G \<turnstile> ?I {(Seqw (Basic (liftl (cmp b))) (lift\<^sub>c c))*} ?I"
-    using assms 
-    apply (intro rules.loop rules.seq, unfold valid_def)
-    apply force
-     apply force
-    apply (rule cmp_sound)
-      apply blast
-     apply (auto simp:)
-    using stabilize_entail by blast
-qed (insert assms, auto, rule stabilize_entail)
-
-
-text \<open>Do While Rule\<close>
-lemma do_wp:
-  assumes "R,G \<turnstile>\<^sub>w stabilize R J {c} stabilize R (wp\<^sub>i (cmp b) (stabilize R J) \<inter> (wp\<^sub>i (ncmp b) Q))" (is "R,G \<turnstile>\<^sub>w ?I {c} ?Q")
-  shows "R,G \<turnstile>\<^sub>w stabilize R J {DoWhile J c b} Q"
-  unfolding valid_def lift\<^sub>c.simps
-  sorry
-(*
-proof (intro impI conjI rules.choice rules.seq)
-  assume "wellformed R G \<and> stable\<^sub>t R Q \<and> guar\<^sub>c (DoWhile J c b) (G)"
-  thus "step\<^sub>t R,step G \<turnstile> ?I {lift\<^sub>c c} ?Q" 
-    using assms by (auto simp: valid_def) 
-next
-  assume "wellformed R G \<and> stable\<^sub>t R Q \<and> guar\<^sub>c (DoWhile J c b) (G)"
-  thus "step\<^sub>t R,step G \<turnstile> ?I {(lift\<^sub>c c ;; Basic (\<lfloor>cmp b\<rfloor>))*} ?I"
-    using assms
-    apply (intro rules.loop rules.seq)
-    prefer 2
-    apply auto[1]
+  hence "base_rel_rely (step\<^sub>t R),base_rel_guar (step G) w \<turnstile> 
+      spec_pred_of_lvm_pred P w {\<triangle> Capture (emptyFrame w) r} spec_pred_of_lvm_pred Q w"
+    apply (rule conseq)
+       apply blast+
+    using wf(2)
+    apply (rule base_rel)
     apply blast
-    unfolding valid_def
-    apply (simp add: rules.intros(8) stabilize_entail stabilize_stable subsetI)
-    apply (subgoal_tac "stable\<^sub>t R
-     (stabilize R
-       ({m. ((st_ev\<^sub>B m b) \<longrightarrow> (m \<in> (stabilize R J)))} \<inter>
-        {m. ((\<not> (st_ev\<^sub>B m b)) \<longrightarrow> (m \<in> Q))}))")
-    apply clarsimp
-    apply (rule rules.conseq)
-    apply blast
-    apply blast
-    apply blast
-    apply blast
-    defer 1
-    apply blast
-    using stabilize_entail by auto
-qed (insert assms, auto, rule stabilize_entail, auto)
-*)
+    done
 
-
-text \<open>False Rule\<close>
-lemma false_wp:
-  assumes "P = ({}, {})"
-  shows "R,G \<turnstile>\<^sub>w P {c} Q"
-  using assms unfolding valid_def
-  by (intro conjI impI rules.conseq[OF falseI, where ?G="step G"]) (auto)
-
-
-text \<open>Rewrite Rule\<close>
-lemma rewrite_wp:
-  "R,G \<turnstile>\<^sub>w P {c} Q \<Longrightarrow> R,G \<turnstile>\<^sub>w M \<ge> P \<Longrightarrow> R,G \<turnstile>\<^sub>w M {c} Q"
-  by (auto simp: valid_def context_order_def)
-
-text \<open>Assert Rule\<close>
-lemma assert_wp:
-  assumes "A \<Longrightarrow> R,G \<turnstile>\<^sub>w P {c} Q"
-  shows "R,G \<turnstile>\<^sub>w (P \<inter> assert A) {c} Q"
-proof (cases A)
-  case True
-  then show ?thesis using assms by (intro rewrite_wp[OF _ assert_ord], simp)
-next
-  case False
-  then show ?thesis by (intro false_wp, auto simp: assert_def)
-qed 
-
-
-*)
-
+  thus ?thesis by auto
+qed
 
 lemma [simp]:
   "(a \<union> b) \<inter> w = (a \<inter> w \<union> b \<inter> w)"
   by auto
 
 
+text \<open>Ensure all global operations in a thread conform to its guarantee\<close>
+fun guarl
+  where 
+    "guarl w Skip G = True" |
+    "guarl w (Op v a f) G = (v\<^sup>U \<subseteq> guar (wp\<^sub>i a o wp\<^sub>a f) (step G) \<and> (\<forall>m. v \<subseteq> {s. s \<in> wp\<^sub>i\<^sub>s a
+                     {t'.
+                      (gl_restrict s\<lparr>varmap_rec.more := m\<rparr>,
+                       gl_restrict t'\<lparr>varmap_rec.more := m\<rparr>)
+                      \<in> id_on w (step G)}}))" |
+    "guarl w (SimAsm.lang.Seq c\<^sub>1 c\<^sub>2) G = (guarl w c\<^sub>1 G \<and> guarl w c\<^sub>2 G)" |
+    "guarl w (If _ c\<^sub>1 c\<^sub>2) G = (guarl w c\<^sub>1 G \<and> guarl w c\<^sub>2 G)" |
+    "guarl w (While _ _ _ c) G = (guarl w c G)" |
+    "guarl w (DoWhile _ _ c _) G = (guarl w c G)"
+
 text \<open>Com Rule\<close>
 theorem com_wp:
-  (* Q captures the speculative implzications of r *)
-  assumes s: "(base_rel_frame_id (step\<^sub>t R)), (base_rel_guar G' w) \<turnstile> (spec_pred_of_lvm_pred [Q]\<^sub>s w) {r} (spec_pred_of_lvm_pred Q' w)"
+  (* Q captures the speculative implications of r *)
+  assumes s: "(base_rel_rely (step\<^sub>t R)), (base_rel_guar (step G) w) \<turnstile> (spec_pred_of_lvm_pred [Q]\<^sub>s w) {r} (spec_pred_of_lvm_pred Q' w)"
   (* Q is stable *)
   assumes st: "stable\<^sub>t R [Q]\<^sub>;" "stable\<^sub>L R [Q]\<^sub>s"
   (* VCs are strong enough to establish guarantee *)
-  assumes g: "guar\<^sub>c c G" "wr\<^sub>l c \<subseteq> w" "lk\<^sub>l c \<inter> w = {}"
-
+  assumes g: "guarl w c G" "wr\<^sub>l c \<subseteq> w" "lk\<^sub>l c \<inter> w = {}"
   (* Standard properties of R G *)
-  assumes wf: "wellformed R G" "reflexive G'" "G' \<subseteq> step\<^sub>t R \<inter> step G"
+  assumes wf: "wellformed R G" "id_on w (step G) \<subseteq> step\<^sub>t R \<inter> step G"
 
-  shows "(R,G,G' \<turnstile> wp R c Q {c,r,w} Q) \<and> (stable\<^sub>t R [wp R c Q]\<^sub>; \<and> stable\<^sub>L R [wp R c Q]\<^sub>s)"
-  using s st g
+  shows "(R,G \<turnstile> wp R c Q {c,r,w} Q) \<and> (stable\<^sub>t R [wp R c Q]\<^sub>; \<and> stable\<^sub>L R [wp R c Q]\<^sub>s)"
+  using s st g wf(2)
 proof (induct c arbitrary: Q' Q r w)
   case Skip
   then show ?case by (auto)
 next
   case (Op x1 x2 x3)
-  thus ?case using wf by (intro conjI basic_wp) auto
+  thus ?case using wf(1) 
+    using basic_wp[OF wf(1) _ _ Op(2,3) Op(5)[simplified] Op(6)[simplified]] 
+    by auto
 next
   case (Seq c\<^sub>1 c\<^sub>2)
-  hence c2: "R,G,G' \<turnstile> wp R c\<^sub>2 Q {c\<^sub>2,r,w} Q" "stable\<^sub>t R [wp R c\<^sub>2 Q]\<^sub>;" "stable\<^sub>L R [wp R c\<^sub>2 Q]\<^sub>s" by simp+
-  have "(R,G,G' \<turnstile> wp R c\<^sub>1 (wp R c\<^sub>2 Q) {c\<^sub>1,lift\<^sub>c (ts_lang_of_vm_lang c\<^sub>2) r w,w} (wp R c\<^sub>2 Q))
+  hence c2: "R,G \<turnstile> wp R c\<^sub>2 Q {c\<^sub>2,r,w} Q" "stable\<^sub>t R [wp R c\<^sub>2 Q]\<^sub>;" "stable\<^sub>L R [wp R c\<^sub>2 Q]\<^sub>s" by simp+
+  have "(R,G \<turnstile> wp R c\<^sub>1 (wp R c\<^sub>2 Q) {c\<^sub>1,lift\<^sub>c (ts_lang_of_vm_lang c\<^sub>2) r w,w} (wp R c\<^sub>2 Q))
           \<and> (stable\<^sub>t R [wp R c\<^sub>1 (wp R c\<^sub>2 Q)]\<^sub>; \<and> stable\<^sub>L R [wp R c\<^sub>1 (wp R c\<^sub>2 Q)]\<^sub>s)"
-    using Seq(1)[OF _ c2(2,3)] c2(1) Seq(6,7,8) by auto
+    using Seq(1)[OF _ c2(2,3)] c2(1) Seq(6,7,8,9) by auto
   then show ?case using c2 by auto
 next
   case (If b c\<^sub>1 c\<^sub>2)
-  hence c1: "R,G,G' \<turnstile> wp R c\<^sub>1 Q {c\<^sub>1,r,w} Q" by simp
-  hence c2: "R,G,G' \<turnstile> wp R c\<^sub>2 Q {c\<^sub>2,r,w} Q" using If by simp
+  hence c1: "R,G \<turnstile> wp R c\<^sub>1 Q {c\<^sub>1,r,w} Q" by simp
+  hence c2: "R,G \<turnstile> wp R c\<^sub>2 Q {c\<^sub>2,r,w} Q" using If by simp
   have st: "stable\<^sub>t R [local.wp R c\<^sub>1 Q]\<^sub>;" "stable\<^sub>t R [local.wp R c\<^sub>2 Q]\<^sub>;"  
            "stable\<^sub>L R [local.wp R c\<^sub>1 Q]\<^sub>s" "stable\<^sub>L R [local.wp R c\<^sub>2 Q]\<^sub>s"
     using If by auto
@@ -1267,13 +870,13 @@ next
   proof (clarsimp, intro choice_if conjI, goal_cases left right spec st1 st2 st3)
     case left
     have c: "R,G \<turnstile>\<^sub>; [wp R c\<^sub>1 Q]\<^sub>; {c\<^sub>1,r,w} [Q]\<^sub>;" using c1 by auto
-    have b: "base_rel_frame_id (step\<^sub>t R),base_rel_guar (step G) w \<turnstile>
+    have b: "base_rel_rely (step\<^sub>t R),base_rel_guar (step G) w \<turnstile>
       seq_pred_of_vm_pred (stabilize R (wp\<^sub>i (cmp b) [wp R c\<^sub>1 Q]\<^sub>;)) 
         {Basic (liftl (cmp b))} 
           seq_pred_of_vm_pred [wp R c\<^sub>1 Q]\<^sub>;" (is "?R,?G \<turnstile> ?P { ?b } ?Q")
       using cmp_seq st If wf by blast
 
-    have s: "base_rel_frame_id (step\<^sub>t R),base_rel_guar (step G) w \<turnstile> 
+    have s: "base_rel_rely (step\<^sub>t R),base_rel_guar (step G) w \<turnstile> 
       seq_pred_of_vm_pred 
         (stabilize R ([local.wp R c\<^sub>2 Q]\<^sub>s \<inter> [local.wp R c\<^sub>1 Q]\<^sub>s)\<^sup>U \<inter> stabilize R
           ({s. ev\<^sub>B (varmap_st s) b \<longrightarrow> s \<in> [local.wp R c\<^sub>1 Q]\<^sub>;} \<inter> {s. \<not> ev\<^sub>B (varmap_st s) b \<longrightarrow> s \<in> [local.wp R c\<^sub>2 Q]\<^sub>;})) 
@@ -1282,7 +885,8 @@ next
           apply (rule seq)
       using If apply fastforce
       using c2 apply fastforce
-      using wf apply fastforce
+      using If apply fastforce
+      using If apply fastforce
       using wf stabilize_entail apply fastforce
       using wf stabilize_entail apply (meson inf.cobounded1 stabilizeE subsetD subsetI ul_restrict_mono)
       using wf by blast
@@ -1291,13 +895,13 @@ next
   next
     case right
     have c: "R,G \<turnstile>\<^sub>; [wp R c\<^sub>2 Q]\<^sub>; {c\<^sub>2,r,w} [Q]\<^sub>;" using c2 by auto
-    have b: "base_rel_frame_id (step\<^sub>t R),base_rel_guar (step G) w \<turnstile>
+    have b: "base_rel_rely (step\<^sub>t R),base_rel_guar (step G) w \<turnstile>
       seq_pred_of_vm_pred (stabilize R (wp\<^sub>i (ncmp b) [wp R c\<^sub>2 Q]\<^sub>;)) 
         {Basic (liftl (ncmp b))} 
           seq_pred_of_vm_pred [wp R c\<^sub>2 Q]\<^sub>;" (is "?R,?G \<turnstile> ?P { ?b } ?Q")
       using cmp_seq st If wf by blast
 
-    have s: "base_rel_frame_id (step\<^sub>t R),base_rel_guar (step G) w \<turnstile> 
+    have s: "base_rel_rely (step\<^sub>t R),base_rel_guar (step G) w \<turnstile> 
       seq_pred_of_vm_pred 
         (stabilize R ([local.wp R c\<^sub>2 Q]\<^sub>s \<inter> [local.wp R c\<^sub>1 Q]\<^sub>s)\<^sup>U \<inter> stabilize R
           ({s. ev\<^sub>B (varmap_st s) b \<longrightarrow> s \<in> [local.wp R c\<^sub>1 Q]\<^sub>;} \<inter> {s. \<not> ev\<^sub>B (varmap_st s) b \<longrightarrow> s \<in> [local.wp R c\<^sub>2 Q]\<^sub>;})) 
@@ -1306,7 +910,8 @@ next
           apply (rule seq)
       using If apply fastforce
       using c1 apply fastforce
-      using wf apply fastforce
+      using If apply fastforce
+      using If apply fastforce
       using wf stabilize_entail apply fastforce
       using wf stabilize_entail apply (meson inf.cobounded1 inf.cobounded2 stabilizeE subsetD subsetI ul_restrict_mono)
       using wf by blast
@@ -1314,21 +919,74 @@ next
     show ?case using c b s by (intro seq) (simp; blast)
   next
     case spec
-    then show ?case
-      sorry
+    have c: "R,G \<turnstile>\<^sub>s [wp R c\<^sub>1 Q]\<^sub>s {c\<^sub>1,r,w} [Q]\<^sub>s" using c1 by auto
+    have b: "base_rel_rely (step\<^sub>t R),base_rel_guar (step G) w \<turnstile>
+      spec_pred_of_lvm_pred (stabilize\<^sub>L R (wp\<^sub>i\<^sub>s (cmp b) [wp R c\<^sub>1 Q]\<^sub>s)) w
+        {Basic (liftl (cmp b))} 
+          spec_pred_of_lvm_pred [wp R c\<^sub>1 Q]\<^sub>s w" (is "?R,?G \<turnstile> ?P { ?b } ?Q")
+      using cmp_spec st If wf by blast
+
+    have s: "?R,?G \<turnstile> spec_pred_of_lvm_pred
+                     ([local.wp R c\<^sub>2 Q]\<^sub>s \<inter> [local.wp R c\<^sub>1 Q]\<^sub>s)
+                     w {\<triangle> Capture (emptyFrame w)
+                            (Seqw
+                              (lift\<^sub>c (ts_lang_of_vm_lang c\<^sub>2) r w)
+                              r)} ?P"
+        apply (rule spec_judgement')
+          apply (rule seq)
+      using If apply fastforce
+      using c2 apply fastforce
+      using If apply fastforce
+      using If apply fastforce
+        apply simp
+        apply rule
+        apply (rule stabilize\<^sub>L_entail)
+          prefer 2 using wf apply blast
+      using wf stabilize\<^sub>L_entail  
+         prefer 3
+      apply simp
+        prefer 3
+      using local.wf(1) apply blast
+
+      sorry (* Stability argument *)
+
+
+       show ?case
+         apply (rule seq)
+          apply (rule seq)
+         using c apply blast
+         using b apply blast
+         using s by blast
   next
     case st1
-    thus ?case sorry
+    thus ?case sorry (* Duplicate the above *)
   next
     case st2
-    thus ?case sorry
+    thus ?case 
+      using local.wf(1) by blast 
   next
     case st3
-    thus ?case sorry
+    thus ?case 
+      using st(3) st(4) stable\<^sub>L_def by auto 
   qed
 next
   case (While x1 x2 x3 c)
-  then show ?case sorry
+  show ?case
+    apply (clarsimp)
+    apply (intro conjI)
+    apply (rule seq)
+        apply (rule seq)
+         apply (rule cmp_seq)
+    using wf apply blast
+    using While apply blast
+      apply (rule spec_judgement)
+    apply (rule seq)
+    apply (rule seq)
+    using While apply blast
+             apply (rule conseq)
+                 apply (rule loop)
+    sorry (* Spec invariant here *)
+
 next
   case (DoWhile x1 x2 c x4)
   then show ?case sorry
@@ -1339,17 +997,17 @@ subsection \<open>High-Level Theorem\<close>
 
 text \<open>Soundness lemma for WP reasoning\<close>
 theorem simAsm_wp_sound:
-  assumes wf: "transitive R" "reflexive R" "reflexive G" "reflexive G'" "G' \<subseteq> step\<^sub>t R \<inter> step G"
+  assumes wf: "transitive R" "reflexive R" "reflexive G" "reflexive G'" "id_on (wr\<^sub>l c) (step G) \<subseteq> step\<^sub>t R \<inter> step G"
   assumes st: "stable\<^sub>t R [Q]\<^sub>;" "stable\<^sub>L R [Q]\<^sub>s"
-  assumes g: "guar\<^sub>c c G"
+  assumes g: "guarl (wr\<^sub>l c) c G"
   assumes P: "P \<subseteq>\<^sub>s wp R c Q"
   assumes l: "lk\<^sub>l c \<inter> wr\<^sub>l c = {}"
   shows "\<Turnstile> c SAT [[P]\<^sub>;, R, G, [Q]\<^sub>;]"
 proof -
-  have "\<forall>d>1. base_rel_frame_id (step\<^sub>t R),base_rel_frame_sz (step G) d (wr\<^sub>l c) \<turnstile> 
+  have "base_rel_rely (step\<^sub>t R),base_rel_guar (step G) (wr\<^sub>l c) \<turnstile> 
           spec_pred_of_lvm_pred [Q]\<^sub>s (wr\<^sub>l c) {com.Nil} spec_pred_of_lvm_pred [Q]\<^sub>s (wr\<^sub>l c)"
     using st(2) by auto
-  hence "R,G,G' \<turnstile> wp R c Q {c,Nil,wr\<^sub>l c} Q" 
+  hence "R,G \<turnstile> wp R c Q {c,Nil,wr\<^sub>l c} Q" 
     using com_wp st wf g l by blast
   hence "R,G \<turnstile>\<^sub>; [wp R c Q]\<^sub>; {c,Nil,wr\<^sub>l c} [Q]\<^sub>;" 
     by blast
